CM2_UBOUNDED_dec.v
@@ -6,24 +6,24 @@ Require Import M2.CM2 M2.CM2_facts.
 Section Construction.
 Variable M : Cm2.
 
-Notation multi_step := (CM2.multi_step M).
+Notation steps := (CM2.steps M).
 Notation bounded := (CM2.bounded M).
 Notation step := (CM2.step M).
 Notation reaches := (CM2.reaches M).
 
 
-Definition path k x := map (fun n => multi_step n x) (seq 0 k).
+Definition path k x := map (fun n => steps n x) (seq 0 k).
 
 Lemma path_length {k x} : length (path k x) = k.
 Proof. by rewrite /path map_length seq_length. Qed.
 
-Lemma In_pathE K x oy : In oy (path K x) -> exists k, k < K /\ multi_step k x = oy.
+Lemma In_pathE K x oy : In oy (path K x) -> exists k, k < K /\ steps k x = oy.
 Proof.
   move=> /in_map_iff [k] [<-] /in_seq ?.
   exists k. split; [lia|done].
 Qed.
 
-Lemma In_pathI k x K : k < K -> In (multi_step k x) (path K x).
+Lemma In_pathI k x K : k < K -> In (steps k x) (path K x).
 Proof.
   move=> ?. apply /in_map_iff. exists k. split; first done.
   apply /in_seq. lia.
@@ -54,7 +54,7 @@ Proof.
   by rewrite /= option_bind_iter Hxy.
 Qed.
 
-Lemma path_plus {k k' x} y : multi_step k x = Some y ->
+Lemma path_plus {k k' x} y : steps k x = Some y ->
   path (k+k') x = path k x ++ path k' y.
 Proof.
   move=> Hxy. rewrite /path seq_app map_app /=.
@@ -64,31 +64,31 @@ Proof.
     move=> k' IH. have ->: S k' = k' + 1 by lia.
     by rewrite ?seq_app IH map_app. }
   rewrite map_map. apply: map_ext => - ?.
-  by move: Hxy => /multi_step_plus ->.
+  by move: Hxy => /steps_plus ->.
 Qed.
 
-Lemma path_S_last {k x} : path (S k) x = (path k x) ++ [multi_step k x].
+Lemma path_S_last {k x} : path (S k) x = (path k x) ++ [steps k x].
 Proof. by rewrite /path seq_S map_app. Qed.
 
-Lemma multi_step_loop_mod {K x k} : multi_step (S K) x = Some x ->
-  multi_step k x = multi_step (k mod (S K)) x.
+Lemma steps_loop_mod {K x k} : steps (S K) x = Some x ->
+  steps k x = steps (k mod (S K)) x.
 Proof.
-  rewrite [in multi_step k x](Nat.div_mod_eq k (S K)).
+  rewrite [in steps k x](Nat.div_mod_eq k (S K)).
   move: (k mod (S K)) => k' Hx. elim: (k / S K).
-  - congr multi_step. lia.
+  - congr steps. lia.
   - move=> n IH. have ->: S K * S n + k' = S K + (S K * n + k') by lia.
-    by move: Hx => /multi_step_plus ->.
+    by move: Hx => /steps_plus ->.
 Qed.
 
-Lemma path_loopE K x : In (multi_step K x) (path K x) -> 
-  forall k, In (multi_step k x) (path K x).
+Lemma path_loopE K x : In (steps K x) (path K x) -> 
+  forall k, In (steps k x) (path K x).
 Proof.
   elim: K x; first done.
-  move=> K IH x. rewrite [multi_step _ _]/= option_bind_iter.
+  move=> K IH x. rewrite [steps _ _]/= option_bind_iter.
   case Hxz: (step x) => [z|].
   - move=> H. rewrite (path_S z Hxz) /= in H. case: H.
-    + move=> Hzx k. have /multi_step_loop_mod -> : multi_step (S K) x = Some x.
-      { by rewrite /multi_step /= option_bind_iter Hxz. }
+    + move=> Hzx k. have /steps_loop_mod -> : steps (S K) x = Some x.
+      { by rewrite /steps /= option_bind_iter Hxz. }
       by apply /In_pathI /(Nat.mod_upper_bound k (S K)).
     + rewrite (path_S z Hxz).
       move=> /IH {}IH [|k]; first by left.
@@ -96,19 +96,19 @@ Proof.
   - rewrite iter_None. move=> /in_map_iff [k] [Hk] /in_seq HK.
     move=> k'. have [|Hkk'] : k' < k \/ k <= k' by lia.
     + move=> ?. apply: In_pathI. lia.
-    + move: (Hk) => /(multi_step_k_monotone k') /(_ Hkk') ->.
+    + move: (Hk) => /(steps_k_monotone k') /(_ Hkk') ->.
       rewrite -Hk. apply: In_pathI. lia.
 Qed.
 
 
-Lemma path_loopE' K x : In (multi_step K x) (path K x) -> 
+Lemma path_loopE' K x : In (steps K x) (path K x) -> 
   forall y, reaches x y -> In (Some y) (path K x).
 Proof.
   move=> /path_loopE H y [k] H'. move: (H k).
   by congr In.
 Qed.
 
-Lemma loop_bounded K x : In (multi_step K x) (path K x) -> bounded K x.
+Lemma loop_bounded K x : In (steps K x) (path K x) -> bounded K x.
 Proof.
   move=> /path_loopE' H. 
   exists (map (fun oy => if oy is Some y then y else x) (path K x)).
@@ -117,28 +117,28 @@ Proof.
 Qed.
 
 Lemma path_noloopI k x :
-  ~ In (multi_step k x) (path k x) -> NoDup (path (k + 1) x).
+  ~ In (steps k x) (path k x) -> NoDup (path (k + 1) x).
 Proof.
   elim: k x.
   { move=> ??. constructor; [done| constructor]. }
   move=> k IH x.
-  rewrite path_S_last /multi_step in_app_iff /= -/(multi_step k x).
+  rewrite path_S_last /steps in_app_iff /= -/(steps k x).
   move=> /Decidable.not_or.
-  have [|/IH ?] := In_dec option_Config_eq_dec (multi_step k x) (path k x).
+  have [|/IH ?] := In_dec option_Config_eq_dec (steps k x) (path k x).
   - move=> /path_loopE /(_ (S k)). tauto.
   - move=> [?] ?.
-    apply /(NoDup_Add (a := multi_step (S k) x) (l := path (k + 1) x)).
+    apply /(NoDup_Add (a := steps (S k) x) (l := path (k + 1) x)).
     + rewrite path_S_last.
-      have := Add_app (multi_step (k + 1) x) (path (k + 1) x) [].
+      have := Add_app (steps (k + 1) x) (path (k + 1) x) [].
       congr Add.
-      * congr multi_step. lia.
+      * congr steps. lia.
       * by rewrite app_nil_r.
     + constructor; first done.
       have ->: k + 1 = S k by lia.
       rewrite path_S_last in_app_iff /=. tauto.
 Qed.
 
-Lemma mortal_bounded {K x} : multi_step K x = None -> bounded K x.
+Lemma mortal_bounded {K x} : steps K x = None -> bounded K x.
 Proof.
   move=> HK.
   exists (map (fun oy => if oy is Some y then y else x) (path K x)).
@@ -147,33 +147,33 @@ Proof.
   - move=> Hk. apply /in_map_iff. exists (Some y).
     split; first done.
     rewrite -Hk. by apply: In_pathI.
-  - by move: HK => /(multi_step_k_monotone k) /(_ ltac:(lia)) ->.
+  - by move: HK => /(steps_k_monotone k) /(_ ltac:(lia)) ->.
 Qed.
 
 Lemma In_None_pathE k x :
-  In None (path k x) -> multi_step k x = None.
+  In None (path k x) -> steps k x = None.
 Proof.
-  move=> /In_pathE [k' [?]] /(multi_step_k_monotone k). apply. lia.
+  move=> /In_pathE [k' [?]] /(steps_k_monotone k). apply. lia.
 Qed.
 
 Lemma NoDup_not_bounded {K x y} : 
-  multi_step K x = Some y -> NoDup (path (K + 1) x) -> not (bounded K x).
+  steps K x = Some y -> NoDup (path (K + 1) x) -> not (bounded K x).
 Proof.
   move=> Hxy HK [L [? HL]].
   apply: (pigeonhole option_Config_eq_dec (path (K+1) x) (map Some L)).
   - move=> [z|] /in_map_iff [k] [Hk] /in_seq ?.
     { apply /in_map_iff. exists z. split; first done.
       apply: HL. by exists k. }
-    by move: Hk Hxy => /(multi_step_k_monotone K) /(_ ltac:(lia)) ->.
+    by move: Hk Hxy => /(steps_k_monotone K) /(_ ltac:(lia)) ->.
   - rewrite map_length path_length. lia.
   - done.
 Qed.
 
 Lemma boundedE {K x} : bounded K x ->
-  (In (multi_step K x) (path K x)) + (multi_step K x = None).
+  (In (steps K x) (path K x)) + (steps K x = None).
 Proof.
   move=> HK.
-  case Hy: (multi_step K x) => [y|]; last by right.
+  case Hy: (steps K x) => [y|]; last by right.
   have [?|] := In_dec option_Config_eq_dec (Some y) (path K x).
   { by left. }
   rewrite -Hy. move=> /path_noloopI /NoDup_not_bounded.
@@ -182,7 +182,7 @@ Qed.
 
 Lemma pointwise_decision K x : {bounded K x} + {not (bounded K x)}.
 Proof.
-  case HK: (multi_step K x) => [y|].
+  case HK: (steps K x) => [y|].
   - have [Hy|Hy] := In_dec option_Config_eq_dec (Some y) (path K x).
     + left. apply: loop_bounded. by rewrite HK.
     + right. apply: (NoDup_not_bounded HK).
@@ -190,7 +190,7 @@ Proof.
   - left. by apply: mortal_bounded.
 Qed.
 
-Lemma multi_step_values_bound k x y : multi_step k x = Some y ->
+Lemma steps_values_bound k x y : steps k x = Some y ->
   value1 x <= k + value1 y /\ value1 y <= k + value1 x /\
   value2 x <= k + value2 y /\ value2 y <= k + value2 x.
 Proof.
@@ -204,41 +204,41 @@ Proof.
     + case Hx: (value1 x) => [|?] /IH /=; lia.
 Qed.
 
-Lemma shift_multi_step_a k K p a b :
+Lemma shift_steps_a k K p a b :
   k <= K ->
-  multi_step k (p, (K + a, b)) =
-  match multi_step k (p, (K, b)) with
+  steps k (p, (K + a, b)) =
+  match steps k (p, (K, b)) with
   | Some (p', (a', b')) => Some (p', (a' + a, b'))
   | None => None
   end.
 Proof.
   elim: k K p a b; first done.
   move=> k IH [|K] p a b ?; first by lia.
-  rewrite /multi_step /= ?option_bind_iter /step -/step /=.
+  rewrite /steps /= ?option_bind_iter /step -/step /=.
   case: (nth_error M p); last by rewrite ?iter_None.
   case.
   - move=> c. rewrite -IH; first by lia.
-    congr multi_step. congr (_, (_, _)). lia.
+    congr steps. congr (_, (_, _)). lia.
   - move=> [] q.
     + case: b => [|b]; rewrite -IH; by [|lia].
     + rewrite -IH; by [|lia].
 Qed.
 
-Lemma shift_multi_step_b k K p a b :
+Lemma shift_steps_b k K p a b :
   k <= K ->
-  multi_step k (p, (a, K + b)) =
-  match multi_step k (p, (a, K)) with
+  steps k (p, (a, K + b)) =
+  match steps k (p, (a, K)) with
   | Some (p', (a', b')) => Some (p', (a', b' + b))
   | None => None
   end.
 Proof.
   elim: k K p a b; first done.
   move=> k IH [|K] p a b ?; first by lia.
-  rewrite /multi_step /= ?option_bind_iter /step -/step /=.
+  rewrite /steps /= ?option_bind_iter /step -/step /=.
   case: (nth_error M p); last by rewrite ?iter_None.
   case.
   - move=> c. rewrite -IH; first by lia.
-    congr multi_step. congr (_, (_, _)). lia.
+    congr steps. congr (_, (_, _)). lia.
   - move=> [] q.
     + rewrite -IH; by [|lia].
     + case: a => [|a]; rewrite -IH; by [|lia].
@@ -249,7 +249,7 @@ Lemma shift_path_a K p a b :
   map (fun oy => if oy is Some (p', (a', b')) then Some (p', (a'+a, b')) else None) (path (K+1) (p, (K, b))).
 Proof. 
   rewrite /path map_map. apply: map_ext_in => k /in_seq ?.
-  apply: shift_multi_step_a. lia.
+  apply: shift_steps_a. lia.
 Qed.
 
 Lemma shift_path_b K p a b :
@@ -257,7 +257,7 @@ Lemma shift_path_b K p a b :
   map (fun oy => if oy is Some (p', (a', b')) then Some (p', (a', b'+b)) else None) (path (K+1) (p, (a, K))).
 Proof. 
   rewrite /path map_map. apply: map_ext_in => k /in_seq ?.
-  apply: shift_multi_step_b. lia.
+  apply: shift_steps_b. lia.
 Qed.
 
 Lemma path_NoDup_a_bound K p a b : K <= a -> NoDup (path (K+1) (p, (a, b))) -> NoDup (path (K+1) (p, (K, b))).
@@ -288,16 +288,16 @@ Proof.
       + lia.
     - apply: H; [lia|done]. }
   move=> ? HK. left => x.
-  have [|/path_noloopI] := In_dec option_Config_eq_dec (multi_step K x) (path K x).
+  have [|/path_noloopI] := In_dec option_Config_eq_dec (steps K x) (path K x).
   { by apply: loop_bounded. }
-  case Hz: (multi_step K x) => [z|]; first last.
+  case Hz: (steps K x) => [z|]; first last.
   { move=> _. by apply: mortal_bounded. }
   (* not bounded *)
   move=> Hx. exfalso.
   move: x Hx Hz => [p [a b]] Hx Hz.
   have Hp : not (length M <= p).
   { move=> /nth_error_None HM. move: Hz. have -> : K = S (K - 1) by lia.
-    by rewrite /multi_step /= option_bind_iter /step /= HM iter_None. }
+    by rewrite /steps /= option_bind_iter /step /= HM iter_None. }
   move: Hx Hz.
   (* it suffices to consider configurations up to values K  *)
   wlog: a b z /(a <= K /\ b <= K); first last.
@@ -310,14 +310,14 @@ Proof.
   { move=> H. have [/H|->] : a <= K \/ a = K + (a - K) by lia.
     { by apply. }
     move=> /path_NoDup_a_bound => /(_ ltac:(lia)) /H {H}.
-    rewrite shift_multi_step_a; first done.
-    case: (multi_step K (p, (K, b))) => [y|]; last done.
+    rewrite shift_steps_a; first done.
+    case: (steps K (p, (K, b))) => [y|]; last done.
     move=> H _. by apply: (H y). }
   move=> ?. have [?|->] : b <= K \/ b = K + (b - K) by lia.
   { move=> /H'K H /H. by apply. }
   move=> /path_NoDup_b_bound => /(_ ltac:(lia)) /H'K.
-  rewrite shift_multi_step_b; first done.
-  case: (multi_step K (p, (a, K))) => [y|]; last done.
+  rewrite shift_steps_b; first done.
+  case: (steps K (p, (a, K))) => [y|]; last done.
   move=> H _. by apply: (H y).
 Qed.
 
@@ -329,13 +329,13 @@ Notation l := (length M).
 (* from an arbitrary config arrive at config with at least one large value *)
 Lemma uniform_decision_aux1 x : let n := l*(l+1) in
   (bounded (l*n*n+1) x) +
-  { y | (exists k, k <= l*n*n /\ multi_step k x = Some y) /\ (n <= value1 y \/ n <= value2 y) }.
+  { y | (exists k, k <= l*n*n /\ steps k x = Some y) /\ (n <= value1 y \/ n <= value2 y) }.
 Proof.
   move=> n.
   have [|/path_noloopI Hx] :=
-    In_dec option_Config_eq_dec (multi_step (l*n*n) x) (path (l*n*n) x).
+    In_dec option_Config_eq_dec (steps (l*n*n) x) (path (l*n*n) x).
   { move=> /loop_bounded H. left. apply: (bounded_monotone _ H). lia. }
-  case Hxy: (multi_step (l*n*n+1) x) => [y|]; first last.
+  case Hxy: (steps (l*n*n+1) x) => [y|]; first last.
   { left. by apply: mortal_bounded. }
   right.
   have [/(pigeonhole option_Config_eq_dec)|] := incl_dec option_Config_eq_dec (path (l*n*n+1) x)
@@ -347,8 +347,8 @@ Proof.
     move: H => [/in_map_iff] [k] [Hk] /in_seq ? H.
     have H'z : not (l <= state z).
     { move=> /nth_error_None Hz.
-      have : multi_step (S k) x = None by rewrite /= Hk /= /step Hz.
-      move=> /(multi_step_k_monotone (l*n*n+1)) /(_ ltac:(lia)).
+      have : steps (S k) x = None by rewrite /= Hk /= /step Hz.
+      move=> /(steps_k_monotone (l*n*n+1)) /(_ ltac:(lia)).
       by rewrite Hxy. }
     split. { exists k. split; [lia|done]. }
     suff : not (value1 z < n /\ value2 z < n) by lia.
@@ -357,7 +357,7 @@ Proof.
     apply /in_prod; [|apply /in_prod]; apply /in_seq; lia.
   - move=> [/in_map_iff] H. exfalso.
     move: H => [k] [+ /in_seq ?].
-    move=> /(multi_step_k_monotone (l*n*n+1)) /(_ ltac:(lia)).
+    move=> /(steps_k_monotone (l*n*n+1)) /(_ ltac:(lia)).
     by rewrite Hxy.
 Qed.
 
@@ -371,38 +371,38 @@ Proof.
   - exists x. by split; [left|tauto].
 Qed.
 
-Lemma shift_multi_step_k_b k p a b n : 
-  multi_step k (p, (a, k)) = Some (p, (a, b)) ->
-  forall i, i <= n -> multi_step (i*k) (p, (a, n*k)) = Some (p, (a, i*b + (n-i)*k)).
+Lemma shift_steps_k_b k p a b n : 
+  steps k (p, (a, k)) = Some (p, (a, b)) ->
+  forall i, i <= n -> steps (i*k) (p, (a, n*k)) = Some (p, (a, i*b + (n-i)*k)).
 Proof.
   move=> Hk i.
   have [b' [-> ->]] : exists b', n * k = n * k + b' /\ (n - i) * k = (n - i) * k + b'.
   { exists 0. lia. }
   elim: i n b'. { move=> ???. congr (Some (_, (_, _))). lia. }
   move=> i IH [|n] b' ?; first by lia.
-  rewrite /= /multi_step iter_plus -/(multi_step _ _).
+  rewrite /= /steps iter_plus -/(steps _ _).
   rewrite -?Nat.add_assoc.
-  rewrite shift_multi_step_b; first by lia.
+  rewrite shift_steps_b; first by lia.
   rewrite Hk. have := IH n (b+b') ltac:(lia).
   congr eq.
-  - congr multi_step. congr (_, (_, _)). lia.
+  - congr steps. congr (_, (_, _)). lia.
   - congr (Some (_, (_, _))). lia.
 Qed.
 
 Lemma k_step_iter k p a1 b1 a2 b2 :
   (k <= a1 \/ a1 = a2) -> (k <= b1 \/ b1 = b2) -> 
-  multi_step k (p, (a1, b1)) = Some (p, (a2, b2)) ->
+  steps k (p, (a1, b1)) = Some (p, (a2, b2)) ->
   let ca := if Nat.eq_dec a1 a2 then 0 else 1 in
   let cb := if Nat.eq_dec b1 b2 then 0 else 1 in
   forall i n a b, i <= n ->
-    multi_step (i*k) (p, (a1+ca*(a+n*a1),b1+cb*(b+n*b1))) =
+    steps (i*k) (p, (a1+ca*(a+n*a1),b1+cb*(b+n*b1))) =
       Some (p, (a1+ca*(a+(n-i)*a1+i*a2),b1+cb*(b+(n-i)*b1+i*b2))).
 Proof.
   move=> Ha Hb Hk ca cb. elim.
   { move=> ????. congr (Some (_, (_, _))); lia. }
   move=> i IH [|n] a b; first by lia.
   move=> /(iffRL (Nat.succ_le_mono _ _)) /IH {}IH.
-  rewrite /= /multi_step iter_plus -/(multi_step _ _).
+  rewrite /= /steps iter_plus -/(steps _ _).
   have := IH (a2+a) (b2+b). congr eq; first last.
   { congr (Some (_, (_, _))); lia. }
   congr Nat.iter.
@@ -410,14 +410,14 @@ Proof.
   move: (Nat.eq_dec a1 a2) (Nat.eq_dec b1 b2) => [?|?] [?|?] /=.
   - rewrite ?Nat.add_0_r Hk.
     congr (Some (_, (_, _))); lia.
-  - rewrite shift_multi_step_b; first lia.
+  - rewrite shift_steps_b; first lia.
     rewrite ?Nat.add_0_r Hk.
     congr (Some (_, (_, _))); lia.
-  - rewrite shift_multi_step_a; first lia.
+  - rewrite shift_steps_a; first lia.
     rewrite ?Nat.add_0_r Hk.
     congr (Some (_, (_, _))); lia.
-  - rewrite shift_multi_step_a; first lia.
-    rewrite shift_multi_step_b; first lia.
+  - rewrite shift_steps_a; first lia.
+    rewrite shift_steps_b; first lia.
     rewrite ?Nat.add_0_r Hk.
     congr (Some (_, (_, _))); lia.
 Qed.
@@ -426,7 +426,7 @@ Qed.
 Lemma not_uniformly_boundedI k p a1 b1 a2 b2 :
   (k <= a1 \/ a1 = a2) -> (k <= b1 \/ b1 = b2) -> 
   (a1 <> a2 \/ b1 <> b2) ->
-  multi_step k (p, (a1, b1)) = Some (p, (a2, b2)) ->
+  steps k (p, (a1, b1)) = Some (p, (a2, b2)) ->
   not (uniformly_bounded M).
 Proof.
   move=> /k_step_iter H /H {}H Hab /H /= + [K].
@@ -434,7 +434,7 @@ Proof.
   move Ha: (a1 + _ * _) => a.
   move Hb: (b1 + _ * _) => b.
   move=> {}H /(_ (p, (a, b))) [L [? HL]].
-  have : incl (map (fun i => multi_step (i * k) (p, (a, b))) (seq 0 (K+1))) (map Some L).
+  have : incl (map (fun i => steps (i * k) (p, (a, b))) (seq 0 (K+1))) (map Some L).
   { move=> z /in_map_iff [i] [<- /in_seq ?]. rewrite H; first by lia.
     apply: in_map. apply: HL. exists (i*k). rewrite H; [lia|done]. }
   move=> /(pigeonhole option_Config_eq_dec). apply.
@@ -446,26 +446,26 @@ Proof.
   move: (Nat.eq_dec a1 a2) (Nat.eq_dec b1 b2) => [?|?] [?|?] /=; nia.
 Qed.
 
-Lemma multi_step_sub {i j x y z} :
+Lemma steps_sub {i j x y z} :
   i <= j ->
-  multi_step i x = Some y ->
-  multi_step j x = Some z ->
-  multi_step (j-i) y = Some z.
+  steps i x = Some y ->
+  steps j x = Some z ->
+  steps (j-i) y = Some z.
 Proof.
-  move=> ? Hi. rewrite [in multi_step j x](ltac:(lia) : j = i + (j - i)).
-  by rewrite /multi_step iter_plus -/(multi_step _ _) Hi.
+  move=> ? Hi. rewrite [in steps j x](ltac:(lia) : j = i + (j - i)).
+  by rewrite /steps iter_plus -/(steps _ _) Hi.
 Qed.
 
 (* from a config with the a really large value arrive at config with two large values *)
 Lemma uniform_decision_aux2 x : ({l*(l+1) <= value1 x} + {l*(l+1) <= value2 x}) ->
   (bounded (l*l+1) x) + (not (uniformly_bounded M)) +
-    { y | (exists k, k <= l*l /\ multi_step k x = Some y) /\ (l <= value1 y /\ l <= value2 y) }.
+    { y | (exists k, k <= l*l /\ steps k x = Some y) /\ (l <= value1 y /\ l <= value2 y) }.
 Proof.
   move=> Hlx.
   have [|/path_noloopI Hx] :=
-    In_dec option_Config_eq_dec (multi_step (l*l) x) (path (l*l) x).
+    In_dec option_Config_eq_dec (steps (l*l) x) (path (l*l) x).
   { move=> /loop_bounded H. left. left. apply: (bounded_monotone _ H). lia. }
-  case Hxy: (multi_step (l*l+1) x) => [y|]; first last.
+  case Hxy: (steps (l*l+1) x) => [y|]; first last.
   { left. left. by apply: mortal_bounded. }
   pose P oz := if oz is Some z then 
     (if Hlx then l <= value2 z else l <= value1 z) else True.
@@ -476,7 +476,7 @@ Proof.
   { move=> /(Exists_sig P HP) [[z|]] [Hz /= H'z].
     - right. exists z. move: Hz => /In_pathE [k [? Hk]]. split.
       + exists k. split; [lia|done].
-      + move: Hk => /multi_step_values_bound. clear P HP.
+      + move: Hk => /steps_values_bound. clear P HP.
         case: Hlx H'z => /=; lia.
     - exfalso. by move: Hz Hxy => /In_None_pathE ->. }
   (* all value1 or value2 are smaller than l, not uniformly bounded *)
@@ -486,12 +486,12 @@ Proof.
     (list_prod (seq 0 l) (seq 0 l)).
   { move=> [p c] /in_map_iff [[[p' [a' b']]|]]; first last.
     { move=> [_ /In_pathE].
-      move=> [?] [?] /(multi_step_k_monotone (l * l + 1)) /(_ ltac:(lia)).
+      move=> [?] [?] /(steps_k_monotone (l * l + 1)) /(_ ltac:(lia)).
       by rewrite Hxy. }
     move=> [+ H]. have ? : not (l <= p').
     { move=> /nth_error_None Hp. move: H => /in_map_iff [k] [Hk /in_seq ?].
-      have : multi_step (S k) x = None by rewrite /= Hk /step /= Hp.
-      move=> /(multi_step_k_monotone (l*l+1)) /(_ ltac:(lia)).
+      have : steps (S k) x = None by rewrite /= Hk /step /= Hp.
+      move=> /(steps_k_monotone (l*l+1)) /(_ ltac:(lia)).
       by rewrite Hxy. }
     case: Hlx H'x HP => /= ? H'x HP.
     - move=> [? ?]. subst p c.
@@ -503,10 +503,10 @@ Proof.
   apply: unnest. { rewrite map_length ?prod_length ?seq_length path_length. lia. }
   rewrite /path map_map. move=> /(dup_seq prod_nat_nat_eq_dec) [[i j]].
   move=> [+ ?].
-  case Hi: (multi_step i x) => [[p [a1 b1]]|]; first last.
-  { move: Hi => /(multi_step_k_monotone (l*l+1)) /(_ ltac:(lia)). by rewrite Hxy. }
-  case Hj: (multi_step j x) => [[p' [a2 b2]]|]; first last.
-  { move: Hj => /(multi_step_k_monotone (l*l+1)) /(_ ltac:(lia)). by rewrite Hxy. }
+  case Hi: (steps i x) => [[p [a1 b1]]|]; first last.
+  { move: Hi => /(steps_k_monotone (l*l+1)) /(_ ltac:(lia)). by rewrite Hxy. }
+  case Hj: (steps j x) => [[p' [a2 b2]]|]; first last.
+  { move: Hj => /(steps_k_monotone (l*l+1)) /(_ ltac:(lia)). by rewrite Hxy. }
   clear H'x.
   have ? : not (p = p' /\ a1 = a2 /\ b1 = b2).
   { move=> [? [? ?]]. subst p' a2 b2.
@@ -520,14 +520,14 @@ Proof.
     have ? : a1 <> a2 by lia.
     (* x ->>i (p, (a1, b1)) ->>(j-i) (p, (a2, b2)); a1 >= j-i or b1 >= j-i *)
     have ? : j-i <= a1.
-    { move: Hi => /multi_step_values_bound /=. lia. }
-    move: Hi Hj => /multi_step_sub H /H{H} /(_ ltac:(lia)).
+    { move: Hi => /steps_values_bound /=. lia. }
+    move: Hi Hj => /steps_sub H /H{H} /(_ ltac:(lia)).
     move /not_uniformly_boundedI. apply; lia.
   - move=> [? ?]. subst p' a2.
     have ? : b1 <> b2 by lia.
     have ? : j-i <= b1.
-    { move: Hi => /multi_step_values_bound /=. lia. }
-    move: Hi Hj => /multi_step_sub H /H{H} /(_ ltac:(lia)).
+    { move: Hi => /steps_values_bound /=. lia. }
+    move: Hi Hj => /steps_sub H /H{H} /(_ ltac:(lia)).
     move /not_uniformly_boundedI. apply; lia.
 Qed.
 
@@ -537,9 +537,9 @@ Lemma uniform_decision_aux3 x : l <= value1 x -> l <= value2 x -> (bounded (l+1)
 Proof.
   move=> ??.
   have [|/path_noloopI Hx] :=
-    In_dec option_Config_eq_dec (multi_step (l) x) (path (l) x).
+    In_dec option_Config_eq_dec (steps (l) x) (path (l) x).
   { move=> /loop_bounded H. left. apply: (bounded_monotone _ H). lia. }
-  case Hxy: (multi_step (l+1) x) => [y|]; first last.
+  case Hxy: (steps (l+1) x) => [y|]; first last.
   { left. by apply: mortal_bounded. }
   right. (* not uniformly bounded *)
   have /(pigeonhole Nat.eq_dec) : incl
@@ -547,20 +547,20 @@ Proof.
     (seq 0 l).
   { move=> p /in_map_iff [[[p' [a' b']]|]]; first last.
     { move=> [_ /In_pathE].
-      move=> [?] [?] /(multi_step_k_monotone (l + 1)) /(_ ltac:(lia)).
+      move=> [?] [?] /(steps_k_monotone (l + 1)) /(_ ltac:(lia)).
       by rewrite Hxy. }
     move=> [->] H. apply /in_seq. suff : not (l <= p) by lia.
     move=> /nth_error_None Hp. move: H => /in_map_iff [k] [Hk /in_seq ?].
-    have : multi_step (S k) x = None by rewrite /= Hk /step /= Hp.
-    move=> /(multi_step_k_monotone (l+1)) /(_ ltac:(lia)).
+    have : steps (S k) x = None by rewrite /= Hk /step /= Hp.
+    move=> /(steps_k_monotone (l+1)) /(_ ltac:(lia)).
     by rewrite Hxy. }
   apply: unnest. { rewrite map_length ?seq_length path_length. lia. }
   rewrite /path map_map. move=> /(dup_seq Nat.eq_dec) [[i j]].
   move=> [+ ?].
-  case Hi: (multi_step i x) => [[p [a1 b1]]|]; first last.
-  { move: Hi => /(multi_step_k_monotone (l+1)) /(_ ltac:(lia)). by rewrite Hxy. }
-  case Hj: (multi_step j x) => [[p' [a2 b2]]|]; first last.
-  { move: Hj => /(multi_step_k_monotone (l+1)) /(_ ltac:(lia)). by rewrite Hxy. }
+  case Hi: (steps i x) => [[p [a1 b1]]|]; first last.
+  { move: Hi => /(steps_k_monotone (l+1)) /(_ ltac:(lia)). by rewrite Hxy. }
+  case Hj: (steps j x) => [[p' [a2 b2]]|]; first last.
+  { move: Hj => /(steps_k_monotone (l+1)) /(_ ltac:(lia)). by rewrite Hxy. }
   move=> ?. subst p'.
   have ? : a1 <> a2 \/ b1 <> b2.
   { suff : not (a1 = a2 /\ b1 = b2) by lia. move=> [??]. subst a2 b2.
@@ -570,8 +570,8 @@ Proof.
     move=> /(_ (Some (p, (a1, b1)))). have ->: i + S (j - i - 1) = j by lia.
     rewrite Hi Hj ?count_occ_app /=. case: (option_Config_eq_dec _ _); [lia|done]. }
   have ?: j - i <= a1 /\ j - i <= b1.
-  { move: Hi => /multi_step_values_bound /=. lia. }
-  move: Hi Hj => /multi_step_sub H /H{H} /(_ ltac:(lia)).
+  { move: Hi => /steps_values_bound /=. lia. }
+  move: Hi Hj => /steps_sub H /H{H} /(_ ltac:(lia)).
   move=> /not_uniformly_boundedI. apply; lia.
 Qed.
 
@@ -584,14 +584,14 @@ Proof.
     by case: (state x); rewrite /= iter_None.
 Qed.
 
-Lemma reaches_bounded {K k x y} : multi_step k x = Some y -> bounded K y -> bounded (k+K) x.
+Lemma reaches_bounded {K k x y} : steps k x = Some y -> bounded K y -> bounded (k+K) x.
 Proof.
   move=> Hxy /boundedE [HK|HK].
   - apply: loop_bounded.
-    move: Hxy (Hxy) => /path_plus -> /multi_step_plus ->.
+    move: Hxy (Hxy) => /path_plus -> /steps_plus ->.
     apply /in_app_iff. by right.
   - apply: mortal_bounded.
-    by move: Hxy => /multi_step_plus ->.
+    by move: Hxy => /steps_plus ->.
 Qed.
 
 Lemma uniform_decision : (uniformly_bounded M) + (not (uniformly_bounded M)).
